

# 3-7 定積分の例題【6】

[6]

$$I = \int_0^{\infty} e^{-b^2(x^2 + a^2/x^2)} dx \quad (a \geq 0) \quad \text{--- ④}$$

前項同様、 $a$  に 関して 微分する、

$$\frac{dI}{da} = -2ab^2 \int_0^{\infty} \frac{1}{x^2} e^{-b^2(x^2 + a^2/x^2)} dx$$

$$\frac{d}{da} e^{-b^2(x^2 + a^2/x^2)} = -b^2/x^2 \cdot (2a)$$

$$x = a/t \quad a < x < \infty$$

$$x : 0 \rightarrow \infty$$

$$t : \infty \rightarrow 0$$

$$\frac{dx}{dt} = -\frac{a}{t^2}$$

$$dx = -\frac{a}{t^2} dt$$

$$\frac{dI}{da} = -2ab^2 \int_{\infty}^0 \frac{t^2}{a^2} e^{-b^2((\frac{a}{t})^2 + t^2)} \cdot (-\frac{a}{t^2}) dt$$

$$= 2b^2 \int_0^{\infty} e^{-b^2(b^2/t^2 + t^2)} dt$$

$$= -2b^2 \int_0^{\infty} e^{-b^2(b^2/t^2 + t^2)} dt$$

$$= -2b^2 I$$

$$\therefore \frac{dI}{da} = -2b^2 I$$

$$\frac{dI}{I} = -2b^2 da$$

$$\int \frac{dI}{I} = \int (-2b^2) da$$

$$\log I = -2b^2 a + C$$

$$I = C' e^{-2b^2 a}$$

$a \neq 0$  とおくと

$$C' = I_{(0)} = \int_0^{\infty} e^{-b^2 x^2} dx \quad (2, 18)$$

$$= \frac{\sqrt{\pi}}{2b} \quad (b > 0)$$

$$\therefore \int_0^{\infty} e^{-b^2(x^2 + a^2/x^2)} dx = \frac{\sqrt{\pi}}{2b} e^{-2ab^2} \quad (a > 0, b > 0) \quad \text{--- ⑤}$$

$$= -\frac{\sqrt{\pi}}{2b} e^{-2ab^2} \quad (a > 0, b < 0)$$

この結果より

$$\int_0^{\infty} e^{-c(x^2/a^2 + b^2/x^2)} dx = \frac{a}{2} \sqrt{\frac{\pi}{c}} e^{-2cb/a} \quad (a, b, c > 0)$$

(証明)  $x = at$ ,

$$\frac{dx}{dt} = a$$

$$dx = a dt$$

$$\int_0^{\infty} e^{-c(x^2/a^2 + (b/a)^2 \frac{1}{x^2})} a dt$$

$$= a \int_0^{\infty} e^{-c(x^2/a^2 + (b/a)^2 \frac{1}{x^2})} dt$$

$$= 2\pi \cdot \text{⑤} \text{ において } b = \frac{b}{a}, a = \frac{b}{a} \geq$$

また、同じ形のものを、対称性を用いて

$$\frac{a}{2} \int_0^{\infty} e^{-c(x^2/a^2 + (b/a)^2 \frac{1}{x^2})} dx = \frac{a}{2} \frac{\sqrt{\pi}}{\sqrt{c}} e^{-2 \frac{b}{a} \cdot c}$$

$$= \frac{a}{2} \sqrt{\frac{\pi}{c}} e^{-2cb/a}$$

$$\int_0^{\infty} e^{-c(x^2/a^2 + b^2/x^2)} dx = \frac{a}{2} \sqrt{\frac{\pi}{c}}$$

(証明)

$$\int_0^{\infty} e^{-c(x^2/a^2 + b^2/x^2) + 2cb/a} dx$$

$$= e^{+2cb/a} \int_0^{\infty} e^{-c(x^2/a^2 + b^2/x^2)} dx$$

前項と同様

11

$$\frac{a}{2} \sqrt{\frac{\pi}{c}} e^{-2cb/a}$$

$$= \frac{a}{2} \sqrt{\frac{\pi}{c}}$$

$e^0 \times e^0$  2つの積に相当